>[!example] 
>- Consider a relation <span style="color:#fffd01">R ( A , B , C , D , E , F , G )</span> with the functional dependencies.
>	- <span style="color:#fffd01">A → BC</span>
>	- <span style="color:#fffd01">BC → DE</span> 
>	- <span style="color:#fffd01">D → F</span>
>	- <span style="color:#fffd01">CF → G</span>
>
> ![[Pasted image 20231020090651.png|500]]
>*Hence :-*
>	**<span style="color:#fffd01">A+ = { A, B, C, D, E, F , G }</span>**
>---
> ![[Pasted image 20231020091037.png|500]]
> *Hence :-*
>	**<span style="color:#fffd01">{ B, C }+ = { B, C, D, E, F, G }</span>**








